src/SepTheoryX.v
@@ -1,7 +1,12 @@
 Require Import Heaps.
 Require Import PropX.
+Require Import Env.
+Require Import PropXTac.
 
 Require Import RelationClasses.
+
+Set Implicit Arguments.
+Set Strict Implicit.
 
 Module SepTheoryX (H : Heap).
   Module HT := HeapTheory H.
@@ -10,44 +15,62 @@ Module SepTheoryX (H : Heap).
     Variable pcType : Type.    
     Variable stateType : Type.
 
-    Definition hprop := HT.smem -> PropX pcType stateType.
-
-    Record Hprop : Type := 
-    { prop : hprop
-    ; respects : forall cs G m m', HT.smem_eq m m' -> 
-      valid cs G (prop m --> prop m')
-    }.
-
-    Coercion prop : Hprop >-> hprop.
+    Definition hprop (sos : list Type) := HT.smem -> propX pcType stateType sos.
 
     Variable cs : codeSpec pcType stateType.
+    Require Import List.
     
-    Definition himp (gl gr : Hprop) : Prop :=
-      forall m, valid cs nil ((prop gl) m) -> valid cs nil ((prop gr) m).
-    Definition heq (gl gr : Hprop) : Prop :=
+    Fixpoint forallXify (ls : list Type) : propX pcType stateType ls -> PropX pcType stateType :=
+      match ls with
+        | nil => fun x => x 
+        | a :: b => fun x => forallXify (PropX.ForallX x)
+      end.
+
+    Fixpoint SubstAll dom (m : hlist (fun T => T -> PropX pcType stateType) dom) (p : propX pcType stateType dom) : PropX pcType stateType :=
+      match p in propX _ _ dom 
+        return hlist (fun T => T -> PropX pcType stateType) dom -> PropX pcType stateType
+        with 
+        | Inj _ p => fun _ => Inj p
+        | Cptr _ pc s => fun m => Cptr pc (fun x => SubstAll m (s x))
+        | And _ l r => fun m => And (SubstAll m l) (SubstAll m r)
+        | Or _ l r => fun m => Or (SubstAll m l) (SubstAll m r)
+        | Imply _ l r => fun m => Imply (SubstAll m l) (SubstAll m r)
+
+        | _ => fun _ => Inj True
+      end m.
+
+    Lemma forallXify_subst : forall sos (l : propX pcType stateType sos),
+      (forall m : hlist (fun T => T -> PropX pcType stateType) sos, 
+        interp cs (SubstAll m l))
+      -> interp cs (forallXify l).
+    Admitted.
+
+    Definition himp (gl gr : hprop nil) : Prop :=
+      forall m, interp cs (gl m --> gr m).
+    Definition heq (gl gr : hprop nil) : Prop :=
       himp gl gr /\ himp gr gl.
 
     Global Instance Relf_himp : Reflexive himp.
     Proof.
-      red. unfold himp. firstorder.
+      red. unfold himp. intros. apply Imply_I. econstructor; simpl; auto.
     Qed.
     Global Instance Trans_himp : Transitive himp.
     Proof.
-      red. unfold himp. firstorder.
-    Qed.
+      red. unfold himp. firstorder. apply Imply_I.
+    Admitted.
 
     Global Instance Relf_heq : Reflexive heq.
     Proof.
-      red. unfold heq. firstorder.
-    Qed.
+      red. unfold heq. 
+    Admitted.
     Global Instance Sym_heq : Symmetric heq.
     Proof.
-      red. unfold heq. firstorder.
-    Qed.
+      red. unfold heq. 
+    Admitted.
     Global Instance Trans_heq : Transitive heq.
     Proof.
-      red. unfold heq. firstorder.
-    Qed.
+      red. unfold heq.
+    Admitted.
 
     Theorem heq_himp : forall a b, heq a b -> himp a b.
     Proof.
@@ -81,9 +104,24 @@ Module SepTheoryX (H : Heap).
                end.
 
     (* Definitions *)
-    Definition hemp : hprop :=
-      fun m => PropX.Inj (HT.semp m).
-    
+    Definition inj sos (p : propX pcType stateType sos) : hprop sos :=
+      fun m => PropX.And p (PropX.Inj (HT.semp m)).
+(*    
+    Theorem hinj_respects (p : PropX pcType stateType) : forall cs G m m', 
+      HT.smem_eq m m' -> valid cs G ((hinj p) m --> (hinj p) m').
+    Proof.
+      unfold hinj; intros. eapply Imply_I. eapply And_I.
+      eapply And_E1. econstructor; left; reflexivity.
+      unfold emp, hemp in *. simpl in *. eapply Inj_E. eapply And_E2.
+      econstructor; left; reflexivity. intros; eapply Inj_I. 
+      eapply HT.semp_mor; eauto. symmetry; eassumption. 
+    Qed.
+
+    Definition inj (p : PropX pcType stateType) : Hprop := Build_Hprop _ (hinj_respects p).
+*)
+
+    Definition emp {sos} : hprop sos := inj (PropX.Inj True).
+(*
     Theorem hemp_respects : forall cs G m m', HT.smem_eq m m' -> 
       valid cs G (hemp m --> hemp m').
       intros; goPropX. unfold hemp. eapply Imply_I.
@@ -93,11 +131,13 @@ Module SepTheoryX (H : Heap).
     Qed.
 
     Definition emp : Hprop := Build_Hprop _ hemp_respects.
+*)
 
-    Definition hstar (l r : Hprop) : hprop :=
+    Definition star sos (l r : hprop sos) : hprop sos :=
       fun m => PropX.Exists (fun ml : HT.smem => PropX.Exists (fun mr : HT.smem =>
-        PropX.And (PropX.Inj (HT.split m ml mr)) (And ((prop l) ml) ((prop r) mr)))).
+        PropX.And (PropX.Inj (HT.split m ml mr)) (And (l ml) (r mr)))).
 
+(*
     Theorem hstar_respects (l r : Hprop) : forall cs G m m', HT.smem_eq m m' -> 
       valid cs G ((hstar l r) m --> (hstar l r) m').
     Proof.
@@ -113,30 +153,17 @@ Module SepTheoryX (H : Heap).
     Qed.
 
     Definition star (l r : Hprop) : Hprop := Build_Hprop _ (hstar_respects l r).
+*)
       
-    Definition hinj (p : PropX pcType stateType) : hprop :=
-      fun m => PropX.And p (prop emp m).
-    
-    Theorem hinj_respects (p : PropX pcType stateType) : forall cs G m m', 
-      HT.smem_eq m m' -> valid cs G ((hinj p) m --> (hinj p) m').
-    Proof.
-      unfold hinj; intros. eapply Imply_I. eapply And_I.
-      eapply And_E1. econstructor; left; reflexivity.
-      unfold emp, hemp in *. simpl in *. eapply Inj_E. eapply And_E2.
-      econstructor; left; reflexivity. intros; eapply Inj_I. 
-      eapply HT.semp_mor; eauto. symmetry; eassumption. 
-    Qed.
-
-    Definition inj (p : PropX pcType stateType) : Hprop := Build_Hprop _ (hinj_respects p).
-
-    Definition hcptr (stateMem : stateType -> H.mem) (p : pcType) (t : stateType -> Hprop) : hprop :=
+(*
+    Definition cptr sos (stateMem : stateType -> H.mem) (p : pcType) 
+      (t : stateType -> hprop sos) : hprop sos :=
       fun h => 
         PropX.And 
-          (PropX.Inj (HT.semp h))
+          (emp h)
           (PropX.Cptr p
             (fun x : stateType => PropX.Exists (fun m => 
-              PropX.And (PropX.Inj (HT.satisfies m (stateMem x))) (prop (t x) m)))).
-
+              PropX.And (PropX.Inj (HT.satisfies m (stateMem x))) (t x m)))).
     Theorem hcptr_respects (stateMem : stateType -> H.mem) (p : pcType) (t : stateType -> Hprop) : 
       forall cs G m m', 
         HT.smem_eq m m' -> valid cs G ((hcptr stateMem p t) m --> (hcptr stateMem p t) m').
@@ -151,10 +178,10 @@ Module SepTheoryX (H : Heap).
 
     Definition cptr (stateMem : stateType -> H.mem) (p : pcType) (t : stateType -> Hprop) : Hprop :=
       Build_Hprop _ (hcptr_respects stateMem p t).
-
-    Definition hex (T : Type) (p : T -> Hprop) : hprop :=
-      fun h => PropX.Exists (fun t => prop (p t) h).
-    
+*)
+    Definition ex sos (T : Type) (p : T -> hprop sos) : hprop sos :=
+      fun h => PropX.Exists (fun t => p t h).
+(*    
     Definition hex_respects T (p : T -> Hprop) : forall cs G m m', 
       HT.smem_eq m m' -> valid cs G ((hex _ p) m --> (hex _ p) m').
     Proof.
@@ -167,51 +194,77 @@ Module SepTheoryX (H : Heap).
     Qed.
 
     Definition ex (T : Type) (p : T -> Hprop) : Hprop := Build_Hprop _ (hex_respects T p).
+*)
+
+    Definition hptsto sos (p : H.addr) (v : H.byte) : hprop sos :=
+      fun h => PropX.And (PropX.Inj (HT.smem_get p h = Some v))
+        (PropX.Forall (fun p' =>
+          (PropX.Imply (PropX.Inj (p <> p')) (PropX.Inj (HT.smem_get p' h = None))))).
 
     (** Lemmas **)
 
+    Lemma himp_star_comm : forall P Q, himp (star P Q) (star Q P).
+    Proof.
+      unfold star; doIt. apply Imply_I. eapply Exists_E. econstructor. left; auto.
+      intros. eapply Exists_E. econstructor; left; auto. intros.
+      do 2 eapply Exists_I. repeat eapply And_I.
+      2: eapply And_E2; eapply And_E2; econstructor; left; auto.
+      2: eapply And_E1; eapply And_E2; econstructor; left; auto.
+      eapply Imply_E. 2: eapply And_E1; econstructor; left; eauto.
+      eapply Imply_I. eapply Inj_E. econstructor; left; auto. intros.
+      apply HT.split_comm in H. apply Inj_I. auto.
+    Qed.      
+
     Theorem himp_star_comm_p : forall P Q R, himp (star P Q) R -> himp (star Q P) R.
     Proof.
-      doIt. eapply HT.split_comm. auto.
+      doIt. generalize (himp_star_comm Q P). intros. eapply Imply_I. eapply Imply_E.
+      eapply interp_weaken in H. eassumption. specialize (H0 m).
+      eapply Imply_E. eapply interp_weaken in H0. eapply H0. econstructor; left; auto.
     Qed.
     Theorem himp_star_comm_c : forall P Q R, himp R (star P Q) -> himp R (star Q P).
     Proof.
-      doIt. eapply HT.split_comm. auto.
-    Qed.
+    Admitted.
 
     Theorem heq_star_comm : forall P Q R, heq (star P Q) R -> heq (star Q P) R.
     Proof.
       intros.
-      generalize (himp_star_comm_p P Q R).
-      generalize (himp_star_comm_c P Q R).
+      generalize (@himp_star_comm_p P Q R).
+      generalize (@himp_star_comm_c P Q R).
       unfold himp, heq in *. intuition.
     Qed.
   
     Theorem himp_star_assoc_p : forall P Q R S,
       himp (star P (star Q R)) S -> himp (star (star P Q) R) S.
     Proof.
+(*
       doIt. apply HT.split_comm. apply HT.split_comm in H. eapply HT.split_assoc; try eassumption. 
       apply HT.split_comm. eassumption. eapply HT.disjoint_split_join.
       apply HT.disjoint_comm. eapply HT.split_split_disjoint; eauto.
       apply HT.split_comm in H0; eassumption.
-    Qed.
+*)
+    Admitted.
     Theorem himp_star_assoc_c : forall P Q R S, 
       himp S (star P (star Q R)) -> himp S (star (star P Q) R).
     Proof.
+(*
       doIt. eapply HT.split_assoc; eassumption. apply HT.split_comm.
       apply HT.disjoint_split_join. apply HT.disjoint_comm.
       eapply HT.split_split_disjoint. apply HT.split_comm. eassumption. eassumption.
-    Qed.
+*)
+    Admitted.
 
     Theorem heq_star_assoc : forall P Q R S, 
       heq S (star P (star Q R)) -> heq S (star (star P Q) R).
     Proof.
+(*
       intros. generalize (himp_star_assoc_p P Q R S). generalize (himp_star_assoc_c P Q R S).
       firstorder.
-    Qed.
+*)
+    Admitted.
 
     Theorem himp_star_frame : forall P Q R S, himp P Q -> himp R S -> himp (star P R) (star Q S).
     Proof.
+(*
       unfold himp; simpl; intros;
         repeat match goal with
                  | [ H : _ -> _ |- _ ] => apply H; clear H
@@ -219,68 +272,87 @@ Module SepTheoryX (H : Heap).
                end; goPropX.
       apply simplify_bwd in H2. apply simplify_bwd in H3. apply H in H2. apply H0 in H3. doIt.
       assumption.
-    Qed.
+*)
+    Admitted.
 
     Theorem heq_star_frame : forall P Q R S, heq P Q -> heq R S -> heq (star P R) (star Q S).
     Proof.
+(*
       intros; generalize (himp_star_frame P Q R S). generalize (himp_star_frame Q P S R).
       unfold heq in *. intuition.
-    Qed.
+*)
+    Admitted.
 
     Theorem himp_star_emp_p : forall P Q, himp P Q -> himp (star emp P) Q.
     Proof.
+(*
       unfold himp. intros. eapply H. unfold star in *. simpl in *.
       goPropX. apply simplify_bwd in H2. destruct P. simpl in *.
       eapply HT.split_semp in H1; eauto.
       apply simplify_fwd.  eapply Imply_E.  2: eassumption. eapply respects0. symmetry; auto.
-    Qed.
+*)
+    Admitted.
 
     Theorem himp_star_emp_p' : forall P Q, himp (star emp P) Q -> himp P Q.
     Proof.
+(*
       unfold himp. intros. eapply H. unfold star in *. simpl in *.
       goPropX. do 2 eexists. split. eapply HT.split_a_semp_a. split; eauto.
       eapply HT.semp_smem_emp.
-    Qed.
+*)
+    Admitted.
 
     Theorem himp_star_emp_c : forall P Q, himp P Q -> himp P (star emp Q).
     Proof.
+(*
       unfold himp. intros. eapply H in H0. unfold star in *. simpl in *.
       goPropX. do 2 eexists. split. eapply HT.split_a_semp_a. split; eauto.
       eapply HT.semp_smem_emp.
-    Qed.
+*)
+    Admitted.
 
     Theorem himp_star_emp_c' : forall P Q, himp P (star emp Q) -> himp P Q.
     Proof.
+(*
       unfold himp. intros. eapply H in H0. unfold star in *. simpl in *.
       goPropX. apply simplify_bwd in H2. destruct Q. simpl in *.
       eapply HT.split_semp in H1; eauto.
       apply simplify_fwd. unfold interp in *.
       eapply Imply_E. eapply respects0. symmetry; eassumption. auto.
-    Qed.
+*)
+    Admitted.
 
     Theorem heq_star_emp : forall P Q, heq P Q -> heq (star emp P) Q.
     Proof.
+(*
       intros. unfold heq in *; intuition.
       eapply himp_star_emp_p. auto.
       eapply himp_star_emp_c. auto.
-    Qed.
+*)
+    Admitted.
 
     Theorem heq_star_emp' : forall P Q, heq (star emp P) Q -> heq P Q.
     Proof.
+(*
       intros. unfold heq in *; intuition.
       eapply himp_star_emp_p' in H0. auto.
       eapply himp_star_emp_c' in H1. auto.
-    Qed.
+*)
+    Admitted.
 
     Theorem himp_star_cancel : forall P Q R, himp Q R -> himp (star P Q) (star P R).
     Proof.
+(*
       intros. eapply himp_star_frame. reflexivity. auto.
-    Qed.
+*)
+    Admitted.
 
     Theorem heq_star_cancel : forall P Q R, heq Q R -> heq (star P Q) (star P R).
     Proof.
+(*
       intros. eapply heq_star_frame. reflexivity. auto.
-    Qed.
+*)
+    Admitted.
 
   End env.
 End SepTheoryX.
